# ODE Equation

$$ y^{(n)}+p_{n-1}(x)y^{(n-1)}+...+p_1y^{'}+p_0y=r(x)$$

# General Solution
$$y(x)=y_h+y_p$$

# $y_h$ Part
solve the ODE
$$ y^{(n)}+p_{n-1}(x)y^{(n-1)}+...+p_1y^{'}+p_0y=0$$
then we get $y_h$ part
___
# $y_p$ Part

## Method 1 : Undetermined Coefficients

Depend on the from $r(x)$
check the chart


Term of $r(x)$   |  Choice of $y_p$
--------------|-------------
$ke^{\gamma x}$|$Ce^{\gamma x}$
$kx^n (n=1,2...)$|$K_nx^n+K_{n-1}x^{n-1}...+K_1x+K_0$
$kcos(wx)$$\quad$ $ksin(wx)$|$Kcos(wx)+Msin(wx)$
$ke^{\alpha x}cos(wx)$$\quad$  $ke^{\alpha x}cos(wx)$|$e^{\alpha x}(Kcos(wx)+Msin(wx))$

*if $y_p$ and $y_h$ are repeated, multiply $y_p$ by $x$ (or $x^2$ if double-root) until there is no repeat.*

*if $$r(x)=r_1(x)+r_2(x)...+r_n(x)$$*
*then$$y_p=y_{p1}+y_{p2}...+y_{pn}$$*
___

## Wronskian

We can use Wronskian to determine wheter functions are independent or dependet.

> W=$$ \begin{vmatrix} f_1 & f_2 & f_3 & \cdots & f_n \\ f_1^1 & f_2^1 & f_3^1 & \cdots & f_n^1 \\ \vdots & \vdots & \vdots & \ddots & \vdots \\ f_1^{( n-1)} & f_2^{( n-1)} & f_3^{(n-1)} & \cdots & f_n^{(n-1)} \\ \end{vmatrix} $$

> If W $\neq$ 0, they are independent.

> if W = 0, they are dependent.

---
## Method 2:Variation of Parameters

$$y_p(x)=\sum_{k=1}^n y_k(x)\int\frac{W_k(x)}{W(x)}dx$$

### Example
> $$x^3y'''+xy'-y=6x$$

>Solve the $y_h$ part
>Cauchy-Euler Equation
$$m^3-3m^2+3m-1=0$$
get $m_1=1$
devide the equation by $m-1$
get equation
$$m^2-2m+1=0$$
knew that $m_3=m_2=m_1=1$
so  $$y_h=c_1x+c_2xln(x)+c_3xln(x)^2$$ 
(cauchy-euler equation)

>solve the $y_p$ part

>### Method 1 : Undetermined Coefficients
>check the $r(x)$ and the table
>the form of $y_p=K_1x+K_0$
>substitute into ODE
>get$$\begin{cases} y=Ax+B \\ y'=A \\y'''=0 \end{cases}$$
>crash

>### Method 2 : Variation of Parameters
>$$W=\begin{vmatrix}y_1&y_2&y_3\\y_1'&y_2'&y_3'\\y_1''&y_2''&y_3''\end{vmatrix}=
>\begin{vmatrix}x&xln(x)&xln(x)^2\\1&ln(x)+1&ln(x)^2+2ln(x)\\0&\frac{1}{x}&\frac{2ln(x)}{x}+\frac{2}{x}\end{vmatrix}
>=2$$
>$$W_1=\begin{vmatrix}0&y_2&y_3\\0&y_2'&y_3'\\r(x)''&y_2''&y_3''\end{vmatrix}=
>\begin{vmatrix}0&xln(x)&xln(x)^2\\0&ln(x)+1&ln(x)^2+2ln(x)\\\frac{6}{x^2}&\frac{1}{x}&\frac{2ln(x)}{x}+\frac{2}{x}\end{vmatrix}
>=\frac{6}{x}(lnx)^2$$
>$$W_2=\begin{vmatrix}y_1&0&y_3\\y_1'&0&y_3'\\y_1''&r(x)''&y_3''\end{vmatrix}=
>\begin{vmatrix}x&0&xln(x)^2\\1&0&ln(x)^2+2ln(x)\\0&\frac{6}{x^2}&\frac{2ln(x)}{x}+\frac{2}{x}\end{vmatrix}
=-\frac{12}{x}ln(x)$$
>$$W_3=\begin{vmatrix}y_1&y_2&0\\y_1'&y_2'&0\\y_1''&y_2''&r(x)''\end{vmatrix}
>=\frac{6}{x}$$
then
$$y_p=y_1\int\frac{W_1}{W}dx+y_2\int\frac{W_2}{W}dx+y_3\int\frac{W_3}{W}dx$$
$$=x\int\frac{3}{x}(lnx)^2dx-xln(x)\int\frac{6}{x}ln(x)dx+xln(x)^2\int\frac{3}{x}dx$$
$$=3xln(x)^3$$

>$$y=y_h+y_p=c_1x+c_2xln(x)+c_3xln(x)^2+3x(lnx)^3$$